# The-4th-order-Runge-Kutta-method-for-a-2nd-order-ODE
The first example: y'' + 4y - cos(3x) = 0, y(x0) = y(0) = 1, y'(x0) = y'(0) = 2
The second example: y'' - 4y = 0, y(x0) = y(0) = 1, y'(x0) = y'(0) = 2
![The first example](https://github.com/KirillGordievich/The-4th-order-Runge-Kutta-method-for-a-2nd-order-ODE/blob/master/graphs/0_2_1_RungeKutta4.png)
![The first example](https://github.com/KirillGordievich/The-4th-order-Runge-Kutta-method-for-a-2nd-order-ODE/blob/master/graphs/0_5_2_RungeKutta4.png)
